src/automata/epsnfa_triv.lean
@@ -10,7 +10,7 @@ namespace epsnfa.triv
 
 variables {S : Type} [fintype S]
 
-@[derive fintype]
+@[derive fintype, derive decidable_eq]
 inductive U : Type
 | start : U
 | finish : U
@@ -29,7 +29,7 @@ begin
     all_goals { simpa [epsnfa_empty] using a_h},
 end
 
-theorem empty_is_epsnfa_lang : epsnfa_lang (∅ : set (list S)) := by exactI ⟨U, _, epsnfa_empty, epsnfa_empty_eq⟩
+theorem empty_is_epsnfa_lang : epsnfa_lang (∅ : set (list S)) := by exactI ⟨U, _, _, epsnfa_empty, epsnfa_empty_eq⟩
 
 def epsnfa_eps : epsNFA S U := {
     start := U.start,
@@ -58,7 +58,7 @@ begin
         }
     }, {
         rintro hw,
-        refine @go.eps _ _ _ _ _ _ _ U.finish _ _ _,
+        refine go.eps U.finish _ _,
         simp [epsnfa_eps],
         rw [mem_singleton_iff] at hw,
         rw hw,
@@ -66,7 +66,7 @@ begin
     }
 end
 
-theorem eps_is_epsnfa_lang : epsnfa_lang ({[]} : set (list S)) :=  by exactI ⟨U, _, epsnfa_eps, epsnfa_eps_eq⟩
+theorem eps_is_epsnfa_lang : epsnfa_lang ({[]} : set (list S)) :=  by exactI ⟨U, _, _, epsnfa_eps, epsnfa_eps_eq⟩
 
 def epsnfa_one (char : S) : epsNFA S U := {
     start := U.start,
@@ -103,12 +103,12 @@ begin
         rintro hw,
         rw [mem_singleton_iff] at hw,
         rw hw,
-        refine @go.step _ _ _ _ _ char _ _ U.finish _ _ _,
+        refine go.step _ go.finish,
         simp [epsnfa_one],
-        exact go.finish,
     }
 end
 
-theorem one_is_epsnfa_lang {char : S} : epsnfa_lang ({[char]} : set (list S)) := by exactI ⟨U, _, epsnfa_one char, epsnfa_one_eq⟩
+theorem one_is_epsnfa_lang {char : S} : epsnfa_lang ({[char]} : set (list S)) := 
+    by exactI ⟨U, _, _, epsnfa_one char, epsnfa_one_eq⟩
 
 end epsnfa.triv
