src/regular/dfa_to_regex.lean
@@ -1,0 +1,301 @@
+import tactic
+import languages.basic
+import languages.star
+import regular.regex
+import automata.dfa
+import data.set.basic
+import data.finset.basic
+import data.finset.fold
+import data.finset.lattice
+import data.fintype.basic
+import data.set.finite
+
+open languages regex dfa finset list
+
+namespace regex.from_dfa
+
+variables {S Q : Type} [fintype S] [fintype Q] [decidable_eq S] [decidable_eq Q]
+
+variables (set1 : set Q) (set2 : finset Q)
+
+inductive go_restr (dfa : DFA S Q) (allow : finset Q) : Q → list S → Q → Prop
+| finish {q : Q}                    : go_restr q [] q
+| last_step {ch : S} {q nxt : Q}    : nxt = dfa.next q ch → go_restr q [ch] nxt
+| step {head : S} {tail : list S} {q nxt f : Q} :
+    nxt = dfa.next q head → nxt ∈ allow → go_restr nxt tail f → go_restr q (head::tail) f
+
+lemma go_restr_univ (dfa : DFA S Q) {a b : Q} {w : list S}
+    : go dfa a w b ↔ go_restr dfa (fintype.elems Q) a w b :=
+begin
+    split, {
+        intro go_dfa,
+        induction go_dfa, 
+        { exact go_restr.finish }, 
+        { refine go_restr.step rfl (finset.mem_univ _) go_dfa_ih, }
+    }, {
+        intro go_restr_dfa,
+        induction go_restr_dfa, 
+        { exact go.finish },
+        { subst go_restr_dfa_a, refine go.step go.finish },
+        { subst go_restr_dfa_a, refine go.step go_restr_dfa_ih },
+    }
+end
+
+lemma go_restr_subset {dfa : DFA S Q} {a b : Q} {w : list S} {fs1 fs2 : finset Q} :
+    fs1 ⊆ fs2 → go_restr dfa fs1 a w b → go_restr dfa fs2 a w b :=
+begin
+    rintro fsub go_fs1,
+    induction go_fs1, 
+    { exact go_restr.finish },
+    { exact go_restr.last_step go_fs1_a },
+    { convert go_restr.step (go_fs1_a) (fsub go_fs1_a_1) go_fs1_ih }
+end
+
+lemma go_restr_append {dfa : DFA S Q} {a b c : Q} {left right : list S} {allowed : finset Q} :
+    b ∈ allowed → go_restr dfa allowed a left b → go_restr dfa allowed b right c →
+    go_restr dfa allowed a (left ++ right) c :=
+begin
+    rintro b_allowed go_ab go_bc,
+    induction go_ab, {
+        exact go_restr_subset (subset.refl _) go_bc,
+    }, {
+        subst go_ab_a,
+        exact go_restr.step rfl b_allowed go_bc,
+    }, {
+        replace go_bc := go_ab_ih b_allowed go_bc,
+        refine go_restr.step go_ab_a go_ab_a_1 go_bc,
+    }
+end
+
+lemma go_restr_list_join {dfa : DFA S Q} {a : Q} {l : list (list S)} {allowed : finset Q} :
+    a ∈ allowed → (∀ x, x ∈ l → go_restr dfa allowed a x a) → go_restr dfa allowed a (join l) a :=
+begin
+    rintro a_allowed hl,
+    induction l with head tail lst_ih, {
+        simp [go_restr.finish],
+    }, {
+        refine go_restr_append a_allowed (hl head _) (lst_ih _),
+        simp only [mem_cons_iff, true_or, eq_self_iff_true],
+        rintro x xtail,
+        refine hl x _,
+        simp only [xtail, mem_cons_iff, or_true],
+    }
+end
+
+def all_edges (dfa : DFA S Q) (a b : Q) : set (list S) := 
+    (⋃ c : S, if dfa.next a c = b then {[c]} else ∅)
+
+def FW (dfa : DFA S Q) : Q → Q → (list Q) → set (list S)
+| a b []                := if a = b then all_edges dfa a b ∪ {[]} else all_edges dfa a b
+| a b (head :: tail)    := (FW a b tail) ∪ (FW a head tail * kleene_star (FW head head tail) * FW head b tail)
+
+lemma FW_to_go_restr {dfa : DFA S Q} {a b : Q} {allowed : list Q} {w : list S} :
+    w ∈ FW dfa a b allowed → go_restr dfa allowed.to_finset a w b :=
+begin
+    induction allowed with head tail ih generalizing a b w, {
+        intro hw,
+        by_cases h : a = b, {
+            simp [FW, all_edges, h] at hw,
+            rcases hw with hw | ⟨ch, win⟩, {
+                substs hw h,
+                exact go_restr.finish,
+            }, {
+                split_ifs at win, {
+                    simp only [set.mem_singleton_iff] at win,
+                    substs h win,
+                    refine go_restr.last_step h_1.symm,
+                }, {
+                    simpa only [set.mem_empty_eq] using win,
+                }
+            }
+        }, {
+            simp [FW, all_edges, h] at hw,
+            rcases hw with ⟨i, win⟩,
+            split_ifs at win,
+            convert go_restr.last_step h_1.symm,  
+            simpa only [set.mem_empty_eq] using win,
+        }, 
+    }, {
+        intro hw,
+        cases hw, {
+            replace hw := ih hw,
+            refine go_restr_subset _ hw,
+            simp [subset_insert], 
+        }, {
+            rcases hw with ⟨_, right, ⟨left, mid, hleft, hmid, rfl⟩, hright, rfl⟩,
+            replace hleft := ih hleft,
+            replace hright := ih hright,
+            rw [star_eq_list_join] at hmid,
+            rcases hmid with ⟨l, hlist, rfl⟩,
+            have h_head : head ∈ (cons head tail).to_finset, by simp only [mem_insert, true_or, eq_self_iff_true, to_finset_cons],
+            have h_subset : tail.to_finset ⊆ (cons head tail).to_finset, by simp only [subset_insert, to_finset_cons],
+            
+            refine go_restr_append h_head _ (go_restr_subset h_subset hright),
+            refine go_restr_append h_head (go_restr_subset h_subset hleft) _,
+            refine go_restr_list_join h_head _,
+            rintro x xtail,
+            apply go_restr_subset h_subset (ih (hlist x xtail)),
+        }
+    }
+end
+
+-- inductive go_restr (dfa : DFA S Q) (allow : finset Q) : Q → list S → Q → Prop
+-- | finish {q : Q}                    : go_restr q [] q
+-- | last_step {ch : S} {q nxt : Q}    : nxt = dfa.next q ch → go_restr q [ch] nxt
+-- | step {head : S} {tail : list S} {q nxt f : Q} :
+--     nxt = dfa.next q head → nxt ∈ allow → go_restr nxt tail f → go_restr q (head::tail) f
+
+
+lemma go_restr_split {dfa : DFA S Q} {a b s : Q} {allowed : list Q} {w : list S} : 
+    go_restr dfa (s::allowed : list Q).to_finset a w b → 
+    (go_restr dfa allowed.to_finset a w b) ∨
+    (∃ pref (inf : list (list S)) suf, 
+        go_restr dfa allowed.to_finset a pref s ∧ 
+        (∀ x, x ∈ inf → go_restr dfa allowed.to_finset s x s) ∧
+        go_restr dfa allowed.to_finset s suf b ∧
+        pref ++ inf.join ++ suf = w) :=
+begin
+    intro go_ab,
+    induction go_ab with _  _ _ _ nxt_eq  head tail _ nxt _ nxt_eq allow_nxt go_tail ih, {
+        left, exact go_restr.finish,
+    }, {
+        left, exact go_restr.last_step nxt_eq,
+    }, {
+        by_cases nxt = s, {
+            substs h,
+            right,
+            cases ih, {
+                use [[head], [], tail],
+                use [go_restr.last_step nxt_eq, forall_mem_nil _, ih],
+                simp only [join, eq_self_iff_true, and_self, singleton_append],
+            }, {
+                rcases ih with ⟨pref, inf, suf, go_pref, go_inf, go_suf, rfl⟩,
+                use [[head], pref :: inf, suf],
+                use [go_restr.last_step nxt_eq],
+                split, {
+                    rintro x hx,
+                    cases hx, {
+                        rw ← hx at go_pref,
+                        exact go_pref,
+                    }, {
+                        exact go_inf x hx,
+                    }
+                }, {
+                    use go_suf,
+                    simp only [join, cons_append, eq_self_iff_true, list.append_assoc, and_self, singleton_append],
+                }
+            }
+        }, {
+            simp only [h, mem_insert, false_or, to_finset_cons] at allow_nxt,
+            cases ih, {
+                left,
+                refine go_restr.step nxt_eq allow_nxt ih,
+            }, {
+                right,
+                rcases ih with ⟨pref, inf, suf, go_pref, go_inf, go_suf, rfl⟩,
+                use [head :: pref, inf, suf],
+                use [go_restr.step nxt_eq allow_nxt go_pref],
+                use [go_inf, go_suf],
+                simp only [cons_append, eq_self_iff_true, and_self],
+            }
+        }
+    }
+end  
+        
+
+lemma FW_from_go_restr {dfa : DFA S Q} {a b : Q} {allowed : list Q} {w : list S} :
+    go_restr dfa allowed.to_finset a w b → w ∈ FW dfa a b allowed :=
+begin
+    intro go_ab,
+    induction allowed with head tail ih generalizing a b w, {
+        dsimp [FW, all_edges],
+        cases go_ab, {
+            simp, 
+        }, {
+            split_ifs; {
+                simp, use [go_ab_ch], simp [go_ab_a.symm],
+            },                              
+        }, {
+            simpa only [to_finset_nil, not_mem_empty] using go_ab_a_1,
+        }
+    }, {
+        dsimp [FW, all_edges],
+        replace go_ab := go_restr_split go_ab,
+        rcases go_ab with _ | ⟨pref, inf, suf, go_pref, go_inf, go_suf, rfl⟩, {
+            left,
+            exact ih go_ab, 
+        }, {
+            right,
+            use [pref ++ inf.join, suf, pref, inf.join],
+            refine ⟨ih go_pref, _, rfl⟩,
+            apply star_eq_list_join.2 ⟨inf, λ x hx, ih (go_inf x hx), rfl⟩,
+            use ih go_suf,
+        }
+    }
+end 
+
+lemma FW_is_regex {dfa : DFA S Q} {a b : Q} {allowed : list Q} :
+    regex_lang (FW dfa a b allowed) :=
+begin
+    induction allowed with head tail ih generalizing a b, {
+        rw FW,
+        split_ifs;
+        try {apply union_is_regex _ eps_is_regex}; {
+            rw [all_edges, ← set.bUnion_univ],
+            lift (set.univ : set S) to finset S using set.finite.of_fintype set.univ,
+            apply finset_bUnion_is_regex _,
+            exact _inst_3,
+            intros c cx,
+            by_cases hnext : dfa.next a c = b, {
+                simp [hnext],
+                exact one_is_regex,
+            }, {
+                simp [hnext],
+                exact empty_is_regex,
+            },
+            exact _inst_1,
+        },
+    }, {
+        rw FW,
+        have rAB := @ih a b,
+        have rAH := @ih a head,
+        have rHH := @ih head head,
+        have rHB := @ih head b,
+        apply union_is_regex rAB,
+        apply append_is_regex (append_is_regex rAH (star_is_regex rHH)) rHB,
+    }
+end
+
+
+lemma FW_is_DFA {dfa : DFA S Q} {allowed : list Q} (hQ : allowed.to_finset = fintype.elems Q) :
+    (⋃ c ∈ dfa.term, FW dfa dfa.start c allowed) = lang_of_dfa dfa :=
+begin
+    apply set.subset.antisymm, {
+        apply set.bUnion_subset,
+        rintro x x_term w w_fw,
+        refine ⟨x, _, x_term⟩,
+        rw go_restr_univ,
+        rw ← hQ,
+        apply FW_to_go_restr w_fw,
+    }, {
+        rintro w ⟨t, w_go, t_term⟩,
+        refine set.mem_bUnion t_term _,
+        apply FW_from_go_restr,
+        rwa [hQ, ← go_restr_univ],
+    }
+end
+
+theorem dfa_to_regex {L : set (list S)} : dfa_lang L → regex_lang L :=
+begin
+    rintro ⟨Q, fQ, dQ, dfa, rfl⟩,
+    resetI,
+    letI := fQ,
+    rcases to_finset_surjective (fintype.elems Q) with ⟨Qlist, hQ⟩,
+    rw ← FW_is_DFA hQ,
+    lift dfa.term to finset Q using set.finite.of_fintype dfa.term, 
+    apply finset_bUnion_is_regex,
+    rintro c cx,
+    exact FW_is_regex,
+end
+
+end regex.from_dfa
